src/lib/GPU.Conditional.fst
@@ -1,6 +1,7 @@
 module GPU.Conditional
 
 open Pulse.Lib.Pervasives
+open Pulse.Lib.BigStar
 open FStar.Tactics.V2
 
 let if_ (b: bool) (p: slprop): slprop = (cond b p emp)
@@ -8,8 +9,8 @@ let if_ (b: bool) (p: slprop): slprop = (cond b p emp)
 // INTRODUCTION and ELIMINATION RULES
 
 ```pulse
-ghost fn if_intro_true (b: bool) (p: slprop)
-  requires p ** (pure b)
+ghost fn if_intro_true (b: bool { b }) (p: slprop)
+  requires p
   ensures  if_ b p
 {
   rewrite p as if_ b p;
@@ -17,8 +18,8 @@ ghost fn if_intro_true (b: bool) (p: slprop)
 ```
 
 ```pulse
-ghost fn if_intro_false (b: bool) (p: slprop)
-  requires emp ** (pure (not b))
+ghost fn if_intro_false (b: bool { not b }) (p: slprop)
+  requires emp
   ensures  if_ b p
 {
   rewrite emp as if_ b p;
@@ -26,8 +27,8 @@ ghost fn if_intro_false (b: bool) (p: slprop)
 ```
 
 ```pulse
-ghost fn if_elim_true (b: bool) (p: slprop)
-  requires if_ b p ** (pure b)
+ghost fn if_elim_true (b: bool { b }) (p: slprop)
+  requires if_ b p
   ensures  p
 {
   unfold if_ b p;
@@ -36,8 +37,8 @@ ghost fn if_elim_true (b: bool) (p: slprop)
 ```
 
 ```pulse
-ghost fn if_elim_false (b: bool) (p: slprop)
-  requires if_ b p ** (pure (not b))
+ghost fn if_elim_false (b: bool { not b }) (p: slprop)
+  requires if_ b p
   ensures  emp
 {
   unfold if_ b p;
@@ -166,5 +167,51 @@ ghost fn if_rewrite (#b: bool) (#p1 p2: slprop) (#e: (squash b -> squash (p1 == 
   } else {
     ()
   }
+}
+```
+
+// BIGSTAR
+
+// #push-options "--print_implicits --print_bound_var_types"
+
+```pulse
+ghost fn bigstar_if_elim
+  (#u1 : int)
+  (#m: nat)
+  (#n : nat {m <= n})
+  (x : nat { m <= x /\ x < n })
+  (p: nat -> slprop)
+  requires bigstar #u1 m n (fun (i:nat { m <= i /\ i < n }) -> if_ (op_Equality #nat i x) (p i))
+  ensures  p x
+{
+  bigstar_extract m n _ x;
+  bigstar_map #u1 #u1 #m #x #(fun (i: nat { m <= i /\ i < n }) -> _ i) #(fun _ -> emp)
+    (fun (i: nat { m <= i /\ i < x }) -> if_elim_false ((i <: nat) = x) (p (i <: nat)));
+  bigstar_emp_elim #_ #m #x;
+  bigstar_map #u1 #u1 #(x + 1) #n #(fun (i: nat { m <= i /\ i < n }) -> _ i) #(fun _ -> emp)
+    (fun (i: nat { (x + 1) <= i /\ i < n }) -> if_elim_false ((i <: nat) = x) (p (i <: nat)));
+  bigstar_emp_elim #_ #(x + 1) #n;
+  if_elim_true true (p x)
+}
+```
+
+```pulse
+ghost fn bigstar_if_intro
+  (#[exact (`0)]u1 : int)
+  (m: nat)
+  (n : nat {m <= n})
+  (x : nat { m <= x /\ x < n })
+  (p: nat -> slprop)
+  requires p x
+  ensures  bigstar #u1 m n (fun (i:nat { m <= i /\ i < n }) -> if_ (op_Equality #nat i x) (p i))
+{
+  if_intro_true true (p x);
+  bigstar_emp_intro u1 m x;
+  bigstar_map #u1 #u1 #m #x #(fun _ -> emp) #(fun (i: nat { m <= i /\ i < x }) -> _ i) 
+    (fun (i: nat { m <= i /\ i < x }) -> if_intro_false ((i <: nat) = x) (p (i <: nat)));
+  bigstar_emp_intro u1 (x + 1) n;
+  bigstar_map #u1 #u1 #(x + 1) #n #(fun _ -> emp) #(fun (i: nat { (x + 1) <= i /\ i < n }) -> _ i) 
+    (fun (i: nat { (x + 1) <= i /\ i < n }) -> if_intro_false ((i <: nat) = x) (p (i <: nat)));
+  bigstar_compose #u1 m n (fun (i:nat { m <= i /\ i < n }) -> if_ (op_Equality #nat i x) (p i)) x;
 }
 ```
