src/lib/GPU.MatrixBarrier.fsti
@@ -1,0 +1,108 @@
+module GPU.MatrixBarrier
+
+open Pulse.Lib.Pervasives
+open Pulse.Lib.BigStar
+open FStar.Tactics.V2
+open GPU.Base
+module B = GPU.Barrier2
+
+let mbarrier_tok
+  (#n:nat)
+  (p : (it:nat -> from: nat { 0 <= from /\ from < n } -> to: nat { 0 <= to /\ to < n } -> slprop))
+  (b : B.barrier n)
+  (it : nat)
+  (tid : nat { 0 <= tid /\ tid < n })
+  : slprop = B.barrier_tok #n
+    (fun it (from : nat { 0 <= from /\ from < n }) -> bigstar 0 n (p it from))
+    (fun it (to : nat { 0 <= to /\ to < n }) -> bigstar 0 n (fun (from : nat { 0 <= from /\ from < n }) -> p it from to)) b it tid
+
+```pulse
+ghost
+fn mk_mbarrier_proof
+  (n : nat)
+  (p : (it:nat -> from: nat { 0 <= from /\ from < n } -> to: nat { 0 <= to /\ to < n } -> slprop))
+  (it: nat)
+  requires bigstar 0 n (fun (from : nat { 0 <= from /\ from < n }) -> bigstar 0 n (p it from))
+  ensures  bigstar 0 n (fun (to : nat { 0 <= to /\ to < n }) -> bigstar 0 n (fun (from : nat { 0 <= from /\ from < n }) -> p it from to))
+{
+  bigstar_map #0 #0 #0 #n #(fun (from : nat { 0 <= from /\ from < n }) -> bigstar 0 n (p it from)) #_
+    (fun (from : nat { 0 <= from /\ from < n }) -> bigstar_eta _);
+  bigstar_commute #0 #0 0 n 0 n (fun (from : nat { 0 <= from /\ from < n }) -> fun (to : nat { 0 <= to /\ to < n }) -> p it from to);
+}
+```
+
+// TODO: remove
+```pulse
+ghost fn fold_mbarrier_tok
+  (#n:nat)
+  (p : (it:nat -> from: nat { 0 <= from /\ from < n } -> to: nat { 0 <= to /\ to < n } -> slprop))
+  (b : B.barrier n)
+  (it : nat)
+  (tid : nat { 0 <= tid /\ tid < n })
+  requires B.barrier_tok #n
+    (fun it (from : nat { 0 <= from /\ from < n }) -> bigstar 0 n (p it from))
+    (fun it (to : nat { 0 <= to /\ to < n }) -> bigstar 0 n (fun (from : nat { 0 <= from /\ from < n }) -> p it from to)) b it tid
+  ensures mbarrier_tok #n p b it tid
+{
+  fold (mbarrier_tok #n p b it tid)
+}
+```
+
+```pulse
+ghost
+fn mk_mbarrier
+  (n : nat)
+  (p : (it:nat -> from: nat { 0 <= from /\ from < n } -> to: nat { 0 <= to /\ to < n } -> slprop))
+  requires emp
+  returns  b : erased (B.barrier n)
+  ensures  bigstar 0 n (mbarrier_tok p b 0)
+{
+  let b = B.mk_barrier n
+    (fun it (from : nat { 0 <= from /\ from < n }) -> bigstar 0 n (p it from))
+    (fun it (to : nat { 0 <= to /\ to < n }) -> bigstar 0 n (fun (from : nat { 0 <= from /\ from < n }) -> p it from to))
+    (mk_mbarrier_proof n p);
+  bigstar_map #0 #0 #0 #n (fold_mbarrier_tok #n p b 0);
+  b
+}
+```
+
+// __syncthreads()
+```pulse
+fn mbarrier_wait
+  (#n : erased nat)
+  (#p : (it:nat -> from: nat { 0 <= from /\ from < n } -> to: nat { 0 <= to /\ to < n } -> slprop))
+  (b : B.barrier n)
+  (#it : erased nat)
+  (#tid : erased nat { tid < n })
+  requires mbarrier_tok p b  it    tid ** bigstar 0 n (p it tid)
+  ensures  mbarrier_tok p b (it+1) tid ** bigstar 0 n (fun (from: nat { 0 <= from /\ from < n }) -> p it from tid)
+{
+  unfold mbarrier_tok;
+  B.barrier_wait #n #(fun it (from: nat { 0 <= from /\ from < n }) -> bigstar 0 n (p it from)) #_ b;
+  fold (mbarrier_tok p b (it+1) tid);
+}
+```
+
+```pulse
+ghost
+val
+fn drop_mbarrier
+  (#n : nat)
+  (#p : (it:nat -> from: nat { from < n } -> to: nat { to < n } -> slprop))
+  (#b : B.barrier n)
+  (#it: nat)
+  requires bigstar 0 n (mbarrier_tok p b it)
+  ensures  emp
+```
+
+(* Does this always deadlock? *)
+// if (tid % 2) {
+//   ...
+//   __syncthreads();
+// } else {
+//   ...
+//   __syncthreads();
+// }
+
+
+
