src/lib/GPU.fsti
@@ -4,4 +4,5 @@ include GPU.Base
 include GPU.Ref
 include GPU.Array
 include GPU.Barrier2
+include GPU.MatrixBarrier
 include GPU.Conditional
